\documentclass[12pt, letterpaper]{article}
\title{0.2 Keep On Factoring Homework}
\usepackage{setspace}
\author{Jacob Zante}
\date{September 5th, 2024}
\doublespacing
\begin{document}
\maketitle

\textbf{Factor completely:} \\
\begin{math}
    \textbf{1)} \hspace{4.5mm} 12x^2y^3 - 18x^3y^2 - 24x^2y^2 \\
    = \hspace{3.5mm} 6x^2y^2(2y - 3x - 4) \\
    \\
    \textbf{2)} \hspace{4.5mm} \frac{1}{4}m^{-2}n^3 + \frac{1}{2}m^5n \\
    = \hspace{3.5mm} \frac{1}{4}m^{-2}n(n^2 + 2m^7) \\
    \\
    \textbf{3)} \hspace{4.5mm} 4t(m + n) + 5s(m + n) \\
    = \hspace{3.5mm} (m + n)(4t + 5s) \\
    \\
    \textbf{4)} \hspace{4.5mm} (x + 2)(x - 2) + 3(x + 2) \\
    = \hspace{3.5mm} (x + 2)((x - 2) + 3) \\
    = \hspace{3.5mm} (x + 2)(x + 1) \\
    \\
    \textbf{5)} \hspace{4.5mm} (x + 3)^2 - 2(x + 3) \\
    = \hspace{3.5mm} (x + 3)((x + 3) - 2) \\
    = \hspace{3.5mm} (x + 3)(x + 1) \\
    \\
    \textbf{6)} \hspace{4.5mm} y^2 + 1 - y^3 - y \\
    = \hspace{3.5mm} -y^3 + y^2 - y + 1 \\
    = \hspace{3.5mm} -y^2(y - 1) - 1(y - 1) \\
    = \hspace{3.5mm} (y - 1)(y^2 - 1) \\
    \\
    \textbf{7)} \hspace{4.5mm} a^2 + 6bc - 3ac - 2ab \\
    = \hspace{3.5mm} \\
    \textbf{8)} \hspace{4.5mm} a^2b^2 - 7ba^2 + 6a^2 - 4b^2 + 28b - 24 \\
    = \hspace{3.5mm} \\
    \textbf{9)} \hspace{4.5mm} n^2 - 10n + 16 \\
    = \hspace{3.5mm} \\
    \textbf{10)} \hspace{2mm} 4t^2 - 13t + 10 \\
    = \hspace{3.5mm} \\
    \textbf{11)} \hspace{2mm} 6w^2 + 13w - 28 \\
    = \hspace{3.5mm} \\
    \textbf{12)} \hspace{2mm} 12x^2 - 2x - 30 \\
    = \hspace{3.5mm} \\
    \textbf{13)} \hspace{2mm} 49s^2 - 56st + 16t^2 \\
    = \hspace{3.5mm} \\
    \textbf{14)} \hspace{2mm} 100m^2 - 121n^2 \\
    = \hspace{3.5mm} \\
    \textbf{15)} \hspace{2mm} 36x^6 - 25y^4 \\
    = \hspace{3.5mm} \\
    \textbf{16)} \hspace{2mm} x^2 + 6xy + 9y^2 - 36 \\
    = \hspace{3.5mm} \\
    \textbf{17)} \hspace{2mm} 25y^2 - 30y + 9 - 4c^2 - 4cd - d^2 \\
    = \hspace{3.5mm} \\
    \textbf{18)} \hspace{2mm} 8a^2 - 32 \\
    = \hspace{3.5mm} \\
    \textbf{19)} \hspace{2mm} x^{4n} - y^{6n} \\
    = \hspace{3.5mm} \\
    \textbf{20)} \hspace{2mm} -4xy^2 - 4xy - x \\
    = \hspace{3.5mm} \\
\end{math}


\end{document}