\documentclass[14pt, a4paper]{extarticle}
\title{Diagnostic questions 8-13}
\usepackage{setspace}
\usepackage[a4paper, total={7.5in, 12in}]{geometry}
\usepackage{amsmath}
\author{Jacob Zante}
\date{September 8th, 2024}
\doublespacing
\begin{document}
\maketitle
\begin{math}
    \text{9. Simplify and state the restrictions for } \frac{3x^2 - 5x - 2}{3x^2 + 13x + 4} \div \frac{x^2 - x - 2}{x^2 + 3x - 4} \\
    = \hspace{3.5mm} \frac{(x - 2)(3x + 1)}{(3x + 1)(x + 4)} \div \frac{(x - 2)(x + 1)}{(x + 4)(x - 1)} \\
    = \hspace{3.5mm} \frac{x - 2}{x + 4} \div \frac{(x - 2)(x + 1)}{(x + 4)(x - 1)} \\
    = \hspace{3.5mm} \frac{(x - 2)(x + 4)(x - 1)}{(x + 4)(x - 2)(x + 1)} \\
    = \hspace{3.5mm} \frac{x - 1}{x + 1} \\
    \\
    \indent \text{10. Determine the equivalent to } \frac{x}{3x - 6} - \frac{3}{2x - 4} \\
    = \hspace{3.5mm} \frac{x(2x - 4)}{(3x - 6)(2x - 4)} - \frac{3(3x - 6)}{(2x - 4)(3x - 6)} \\
    = \hspace{3.5mm} \frac{2x^2 - 4x}{(3x - 6)(2x - 4)} - \frac{9x - 18}{(2x - 4)(3x - 6)} \\
    = \hspace{3.5mm} \frac{2x^2 - 13x - 18}{(3x - 6)(2x - 4)} \\
    \\
    \indent \text{11. Simplify } (2x^4 - 2x^2 - 7) - (3x^4 - x^3 + x^2 - 4) + (x^4 - x^3 + 2x^2 - 1) \\
    = \hspace{3.5mm} 2x^4 - 2x^2 - 7 - 3x^4 + x^3 - x^2 + 4 + x^4 - x^3 + 2x^2 - 1 \\
    = \hspace{3.5mm} -x^2 - 4 \\
    \\
    \indent \text{12. Simplify } (x^2 - 2x - 1) + (3x^2 + x + 2) \\
    = \hspace{3.5mm} 4x^2 - x + 1 \\
    \\
    \indent \text{13. Simplify } -2x(x + 1)^2 + 3x(x - 4) \\
    = \hspace{3.5mm} -2x^3 - 4x^2 - 2x + 3x^2 - 12x \\
    = \hspace{3.5mm} -2x^3 - x^2 - 14x \\
\end{math}


\end{document}